\documentclass{ximeraXloud}
\title{Simplifying Numeric Exponentials}



\begin{document}
\input{Useful-Sage-Macros}

\begin{sagesilent}

##### Problem p1
p1b1 = RandInt(2,7)
p1pwr1 = RandInt(0,5)
p1ans1 = p1b1^p1pwr1
p1ans2 = p1b1^(-p1pwr1)

##### Problem p2
p2b1 = NonZeroInt(2,7,[p1b1])
p2pwr1 = RandInt(0,5)
p2ans1 = p2b1^p2pwr1
p2ans2 = p2b1^(-p2pwr1)

##### Problem p3
p3b1 = NonZeroInt(2,7,[p1b1,p2b1])
p3pwr1 = RandInt(0,5)
p3ans1 = p3b1^p3pwr1
p3ans2 = p3b1^(-p3pwr1)

##### Problem p4
p4b1 = NonZeroInt(2,7,[p1b1,p2b1,p3b1])
p4pwr1 = RandInt(0,5)
p4ans1 = p4b1^p4pwr1
p4ans2 = p4b1^(-p4pwr1)




\end{sagesilent}

\begin{problem}
Compute the following numeric exponential value.

\begin{itemize}
    \item $\sage{p1b1}^{\sage{p1pwr1}} = \answer{\sage{p1ans1}}$
    
    \item $\left(\frac{1}{\sage{p1b1}}\right)^{\sage{p1pwr1}} = \answer{\sage{p1ans2}}$
    
    \item $\left(\sage{p1b1}\right)^{-\sage{p1pwr1}} = \answer{\sage{p1ans2}}$
    
    \item $\left(\frac{1}{\sage{p1b1}}\right)^{-\sage{p1pwr1}} = \answer{\sage{p1ans1}}$

\end{itemize}

\end{problem}

\begin{problem}
Compute the following numeric exponential value.

\begin{itemize}
    \item $\sage{p2b1}^{\sage{p2pwr1}} = \answer{\sage{p2ans1}}$
    
    \item $\left(\frac{1}{\sage{p2b1}}\right)^{\sage{p2pwr1}} = \answer{\sage{p2ans2}}$
    
    \item $\left(\sage{p2b1}\right)^{-\sage{p2pwr1}} = \answer{\sage{p2ans2}}$
    
    \item $\left(\frac{1}{\sage{p2b1}}\right)^{-\sage{p2pwr1}} = \answer{\sage{p2ans1}}$

\end{itemize}

\end{problem}


\begin{problem}
Compute the following numeric exponential value.

\begin{itemize}
    \item $\sage{p3b1}^{\sage{p3pwr1}} = \answer{\sage{p3ans1}}$
    
    \item $\left(\frac{1}{\sage{p3b1}}\right)^{\sage{p3pwr1}} = \answer{\sage{p3ans2}}$
    
    \item $\left(\sage{p3b1}\right)^{-\sage{p3pwr1}} = \answer{\sage{p3ans2}}$
    
    \item $\left(\frac{1}{\sage{p3b1}}\right)^{-\sage{p3pwr1}} = \answer{\sage{p3ans1}}$

\end{itemize}

\end{problem}


\begin{problem}
Compute the following numeric exponential value.

\begin{itemize}
    \item $\sage{p4b1}^{\sage{p4pwr1}} = \answer{\sage{p4ans1}}$
    
    \item $\left(\frac{1}{\sage{p4b1}}\right)^{\sage{p4pwr1}} = \answer{\sage{p4ans2}}$
    
    \item $\left(\sage{p4b1}\right)^{-\sage{p4pwr1}} = \answer{\sage{p4ans2}}$
    
    \item $\left(\frac{1}{\sage{p4b1}}\right)^{-\sage{p4pwr1}} = \answer{\sage{p4ans1}}$

\end{itemize}

\end{problem}


\end{document}