\documentclass{ximeraXloud}
\title{Practice Solving Exponential Equations 1}



\begin{document}
\input{Useful-Sage-Macros}

\begin{sagesilent}

###### Problem p1
p1b1 = RandInt(2,7)
p1pwr1 = NonZeroInt(-4,4)
p1pwr2 = NonZeroInt(-4,4)
p1b2 = p1b1^p1pwr1
p1b3 = p1b1^p1pwr2

p1c1 = NonZeroInt(-5,5)
p1c2 = RandInt(-5,5)
p1c3 = NonZeroInt(-5,5,[p1c1*p1pwr1/p1pwr2])
p1c4 = RandInt(-5,5)

p1f1 = p1c1*x + p1c2
p1f2 = p1c3*x + p1c4

p1ans1 = (p1c4*p1pwr2 - p1c2*p1pwr1)/(p1c1*p1pwr1 - p1c3*p1pwr2)


###### Problem p2
p2b1 = RandInt(2,7)
p2pwr1 = NonZeroInt(-4,4)
p2pwr2 = NonZeroInt(-4,4)
p2b2 = p2b1^p2pwr1
p2b3 = p2b1^p2pwr2

p2c1 = NonZeroInt(-5,5)
p2c2 = RandInt(-5,5)
p2c3 = NonZeroInt(-5,5,[p2c1*p2pwr1/p2pwr2])
p2c4 = RandInt(-5,5)

p2f1 = p2c1*x + p2c2
p2f2 = p2c3*x + p2c4

p2ans1 = (p2c4*p2pwr2 - p2c2*p2pwr1)/(p2c1*p2pwr1 - p2c3*p2pwr2)


###### Problem p3
p3b1 = RandInt(2,7)
p3pwr1 = NonZeroInt(-4,4)
p3pwr2 = NonZeroInt(-4,4)
p3b2 = p3b1^p3pwr1
p3b3 = p3b1^p3pwr2

p3c1 = NonZeroInt(-5,5)
p3c2 = RandInt(-5,5)
p3c3 = NonZeroInt(-5,5,[p3c1*p3pwr1/p3pwr2])
p3c4 = RandInt(-5,5)

p3f1 = p3c1*x + p3c2
p3f2 = p3c3*x + p3c4

p3ans1 = (p3c4*p3pwr2 - p3c2*p3pwr1)/(p3c1*p3pwr1 - p3c3*p3pwr2)


###### Problem p4
p4b1 = RandInt(2,7)
p4pwr1 = NonZeroInt(-4,4)
p4pwr2 = NonZeroInt(-4,4)
p4b2 = p4b1^p4pwr1
p4b3 = p4b1^p4pwr2

p4c1 = NonZeroInt(-5,5)
p4c2 = RandInt(-5,5)
p4c3 = NonZeroInt(-5,5,[p4c1*p4pwr1/p4pwr2])
p4c4 = RandInt(-5,5)

p4f1 = p4c1*x + p4c2
p4f2 = p4c3*x + p4c4

p4ans1 = (p4c4*p4pwr2 - p4c2*p4pwr1)/(p4c1*p4pwr1 - p4c3*p4pwr2)

\end{sagesilent}

\begin{problem}
    Solve for $x$ in the following exponential equation:
    \[
        \left(\sage{p1b2}\right)^{\sage{p1f1}} = \left(\sage{p1b3}\right)^{\sage{p1f2}}
    \]

    $x = \answer{\sage{p1ans1}}$.
\end{problem}


\begin{problem}
    Solve for $x$ in the following exponential equation:
    \[
        \left(\sage{p2b2}\right)^{\sage{p2f1}} = \left(\sage{p2b3}\right)^{\sage{p2f2}}
    \]

    $x = \answer{\sage{p2ans1}}$.
\end{problem}


\begin{problem}
    Solve for $x$ in the following exponential equation:
    \[
        \left(\sage{p3b2}\right)^{\sage{p3f1}} = \left(\sage{p3b3}\right)^{\sage{p3f2}}
    \]

    $x = \answer{\sage{p3ans1}}$.
\end{problem}


\begin{problem}
    Solve for $x$ in the following exponential equation:
    \[
        \left(\sage{p4b2}\right)^{\sage{p4f1}} = \left(\sage{p4b3}\right)^{\sage{p4f2}}
    \]

    $x = \answer{\sage{p4ans1}}$.
\end{problem}


\end{document}