\documentclass{ximeraXloud}
\input{../preamble}
\title{Logarithm Practice}

\begin{document}
\begin{abstract}
    Unlimited Practice for Logarithms.
\end{abstract}
\maketitle

\textbf{NOTE:} These are all randomized problems. As a result, it is entirely possible to get pretty awful numbers if you are suitably unlucky. Some of these may look bad until you start doing them, but if you see problems that look excessively awful, remember that you can always hit the `Another' button in the top (green refresh arrow) to get new numbers. If you find yourself doing this frequently, you may want to discuss it with your TA to see if you have a gap in your understanding, or to see if the problems are just really that bad (in which case the TA will forward the info to the content authors).

%\input{Useful-Sage-Macros}

\begin{sagesilent}
#####Define default Sage variables.
#Default function variables
var('x,y,z,X,Y,Z')
#Default function names
var('f,g,h,dx,dy,dz,dh,df')
#Default Wild cards
w0 = SR.wild(0)

def RandInt(a,b):
    """ Returns a random integer in [`a`,`b`]. Note that `a` and `b` should be integers themselves to avoid unexpected behavior.
    """
    return QQ(randint(int(a),int(b)))
    # return choice(range(a,b+1))

def NonZeroInt(b,c, avoid = [0]):
    """ Returns a random integer in [`b`,`c`] which is not in `av`. 
        If `av` is not specified, defaults to a non-zero integer.
    """
    while True:
        a = RandInt(b,c)
        if a not in avoid:
            return a

\end{sagesilent}
\begin{sagesilent}
### Problem p1

p1b1 = NonZeroInt(2,15,[4,8,9])

p1c1 = NonZeroInt(-15,15)
p1c2 = NonZeroInt(-15,15,[0,p1c1])
p1c3 = NonZeroInt(-15,15)
p1c4 = NonZeroInt(-15,15,[0,p1c3])
p1c5 = NonZeroInt(-15,15)
p1c6 = NonZeroInt(-15,15,[0,p1c5])
p1c7 = NonZeroInt(-15,15,[0,p1c1])
p1c8 = NonZeroInt(-15,15,[0,p1c7])
p1c9 = NonZeroInt(-15,15,[0,p1c2])
p1c10 = NonZeroInt(-15,15,[0,p1c9])
p1c11 = NonZeroInt(-15,15,[0,p1c3])
p1c12 = NonZeroInt(-15,15,[0,p1c11])

p1f1 = p1c1*x + p1c2
p1f2 = p1c3*y + p1c4
p1f3 = p1c5*z + p1c6
p1f4 = p1c7*x + p1c8
p1f5 = p1c9*y + p1c10
p1f6 = p1c11*z + p1c12

p1q1 = (p1f1*p1f2^2*p1f3^3)/(p1f4^4*p1f5^5*p1f6^6)



### Problem p2

p2b1 = NonZeroInt(2,15,[4,8,9])

p2c1 = NonZeroInt(-15,15)
p2c2 = NonZeroInt(-15,15,[0,p2c1])
p2c3 = NonZeroInt(-15,15)
p2c4 = NonZeroInt(-15,15,[0,p2c3])
p2c5 = NonZeroInt(-15,15)
p2c6 = NonZeroInt(-15,15,[0,p2c5])
p2c7 = NonZeroInt(-15,15,[0,p2c1])
p2c8 = NonZeroInt(-15,15,[0,p2c7])
p2c9 = NonZeroInt(-15,15,[0,p2c2])
p2c10 = NonZeroInt(-15,15,[0,p2c9])
p2c11 = NonZeroInt(-15,15,[0,p2c3])
p2c12 = NonZeroInt(-15,15,[0,p2c11])

p2f1 = p2c1*x + p2c2
p2f2 = p2c3*y + p2c4
p2f3 = p2c5*z + p2c6
p2f4 = p2c7*x + p2c8
p2f5 = p2c9*y + p2c10
p2f6 = p2c11*z + p2c12

p2q1 = (p2f1*p2f2^2*p2f3^3)/(p2f4^4*p2f5^5*p2f6^6)



### Problem p3

p3b1 = NonZeroInt(2,15,[4,8,9])

p3c1 = NonZeroInt(-15,15)
p3c2 = NonZeroInt(-15,15,[0,p3c1])
p3c3 = NonZeroInt(-15,15)
p3c4 = NonZeroInt(-15,15,[0,p3c3])
p3c5 = NonZeroInt(-15,15)
p3c6 = NonZeroInt(-15,15,[0,p3c5])
p3c7 = NonZeroInt(-15,15,[0,p3c1])
p3c8 = NonZeroInt(-15,15,[0,p3c7])
p3c9 = NonZeroInt(-15,15,[0,p3c2])
p3c10 = NonZeroInt(-15,15,[0,p3c9])
p3c11 = NonZeroInt(-15,15,[0,p3c3])
p3c12 = NonZeroInt(-15,15,[0,p3c11])

p3f1 = p3c1*x + p3c2
p3f2 = p3c3*y + p3c4
p3f3 = p3c5*z + p3c6
p3f4 = p3c7*x + p3c8
p3f5 = p3c9*y + p3c10
p3f6 = p3c11*z + p3c12

p3q1 = (p3f1*p3f2^2*p3f3^3)/(p3f4^4*p3f5^5*p3f6^6)



### Problem p4

p4b1 = NonZeroInt(2,15,[4,8,9])

p4c1 = NonZeroInt(-15,15)
p4c2 = NonZeroInt(-15,15,[0,p4c1])
p4c3 = NonZeroInt(-15,15)
p4c4 = NonZeroInt(-15,15,[0,p4c3])
p4c5 = NonZeroInt(-15,15)
p4c6 = NonZeroInt(-15,15,[0,p4c5])
p4c7 = NonZeroInt(-15,15,[0,p4c1])
p4c8 = NonZeroInt(-15,15,[0,p4c7])
p4c9 = NonZeroInt(-15,15,[0,p4c2])
p4c10 = NonZeroInt(-15,15,[0,p4c9])
p4c11 = NonZeroInt(-15,15,[0,p4c3])
p4c12 = NonZeroInt(-15,15,[0,p4c11])

p4f1 = p4c1*x + p4c2
p4f2 = p4c3*y + p4c4
p4f3 = p4c5*z + p4c6
p4f4 = p4c7*x + p4c8
p4f5 = p4c9*y + p4c10
p4f6 = p4c11*z + p4c12

p4q1 = (p4f1*p4f2^2*p4f3^3)/(p4f4^4*p4f5^5*p4f6^6)



### Problem p5

p5b1 = NonZeroInt(2,15,[4,8,9])

p5c1 = NonZeroInt(-15,15)
p5c2 = NonZeroInt(-15,15,[0,p5c1, 2*p5c1, 3*p5c1, -p5c1, -2*p5c1,-3*p5c1])
p5c3 = NonZeroInt(-15,15)
p5c4 = NonZeroInt(-15,15,[0,p5c3, 2*p5c3, 3*p5c3, -p5c3, -2*p5c3,-3*p5c3])
p5c5 = NonZeroInt(-15,15)
p5c6 = NonZeroInt(-15,15,[0,p5c5, 2*p5c5, 3*p5c5, -p5c5, -2*p5c5,-3*p5c5])
p5c7 = NonZeroInt(-15,15,[0,p5c1])
p5c8 = NonZeroInt(-15,15,[0,p5c7, 2*p5c7, 3*p5c7, -p5c7, -2*p5c7,-3*p5c7])
p5c9 = NonZeroInt(-15,15,[0,p5c2])
p5c10 = NonZeroInt(-15,15,[0,p5c9, 2*p5c9, 3*p5c9, -p5c9, -2*p5c9,-3*p5c9])
p5c11 = NonZeroInt(-15,15,[0,p5c3])
p5c12 = NonZeroInt(-15,15,[0,p5c11, 2*p5c11, 3*p5c11, -p5c11, -2*p5c11,-3*p5c11])

p5f1 = p5c1*x + p5c2
p5f2 = p5c3*y + p5c4
p5f3 = p5c5*z + p5c6
p5f4 = p5c7*x + p5c8
p5f5 = p5c9*y + p5c10
p5f6 = p5c11*z + p5c12

p5cc1 = NonZeroInt(-10,10, [0,1])
p5cc2 = NonZeroInt(-10,10, [0,1])
p5cc3 = NonZeroInt(-10,10, [0,1])
p5cc4 = NonZeroInt(-10,10, [0,1])
p5cc5 = NonZeroInt(-10,10, [0,1])
p5cc6 = NonZeroInt(-10,10, [0,1])

p5a1 = simplify(e^(p5cc1*ln(p5f1)+p5cc2*ln(p5f2)+p5cc3*ln(p5f3)+p5cc4*ln(p5f4)+p5cc5*ln(p5f5)+p5cc6*ln(p5f6)))


### Problem p6

p6b1 = NonZeroInt(2,15,[4,8,9])

p6c1 = NonZeroInt(-15,15)
p6c2 = NonZeroInt(-15,15,[0,p6c1, 2*p6c1, 3*p6c1, -p6c1, -2*p6c1,-3*p6c1])
p6c3 = NonZeroInt(-15,15)
p6c4 = NonZeroInt(-15,15,[0,p6c3, 2*p6c3, 3*p6c3, -p6c3, -2*p6c3,-3*p6c3])
p6c5 = NonZeroInt(-15,15)
p6c6 = NonZeroInt(-15,15,[0,p6c5, 2*p6c5, 3*p6c5, -p6c5, -2*p6c5,-3*p6c5])
p6c7 = NonZeroInt(-15,15,[0,p6c1])
p6c8 = NonZeroInt(-15,15,[0,p6c7, 2*p6c7, 3*p6c7, -p6c7, -2*p6c7,-3*p6c7])
p6c9 = NonZeroInt(-15,15,[0,p6c2])
p6c10 = NonZeroInt(-15,15,[0,p6c9, 2*p6c9, 3*p6c9, -p6c9, -2*p6c9,-3*p6c9])
p6c11 = NonZeroInt(-15,15,[0,p6c3])
p6c12 = NonZeroInt(-15,15,[0,p6c11, 2*p6c11, 3*p6c11, -p6c11, -2*p6c11,-3*p6c11])

p6f1 = p6c1*x + p6c2
p6f2 = p6c3*y + p6c4
p6f3 = p6c5*z + p6c6
p6f4 = p6c7*x + p6c8
p6f5 = p6c9*y + p6c10
p6f6 = p6c11*z + p6c12

p6cc1 = NonZeroInt(-10,10, [0,1])
p6cc2 = NonZeroInt(-10,10, [0,1])
p6cc3 = NonZeroInt(-10,10, [0,1])
p6cc4 = NonZeroInt(-10,10, [0,1])
p6cc5 = NonZeroInt(-10,10, [0,1])
p6cc6 = NonZeroInt(-10,10, [0,1])

p6a1 = simplify(e^(p6cc1*ln(p6f1)+p6cc2*ln(p6f2)+p6cc3*ln(p6f3)+p6cc4*ln(p6f4)+p6cc5*ln(p6f5)+p6cc6*ln(p6f6)))


### Problem p7

p7b1 = NonZeroInt(2,15,[4,8,9])

p7c1 = NonZeroInt(-15,15)
p7c2 = NonZeroInt(-15,15,[0,p7c1, 2*p7c1, 3*p7c1, -p7c1, -2*p7c1,-3*p7c1])
p7c3 = NonZeroInt(-15,15)
p7c4 = NonZeroInt(-15,15,[0,p7c3, 2*p7c3, 3*p7c3, -p7c3, -2*p7c3,-3*p7c3])
p7c5 = NonZeroInt(-15,15)
p7c6 = NonZeroInt(-15,15,[0,p7c5, 2*p7c5, 3*p7c5, -p7c5, -2*p7c5,-3*p7c5])
p7c7 = NonZeroInt(-15,15,[0,p7c1])
p7c8 = NonZeroInt(-15,15,[0,p7c7, 2*p7c7, 3*p7c7, -p7c7, -2*p7c7,-3*p7c7])
p7c9 = NonZeroInt(-15,15,[0,p7c2])
p7c10 = NonZeroInt(-15,15,[0,p7c9, 2*p7c9, 3*p7c9, -p7c9, -2*p7c9,-3*p7c9])
p7c11 = NonZeroInt(-15,15,[0,p7c3])
p7c12 = NonZeroInt(-15,15,[0,p7c11, 2*p7c11, 3*p7c11, -p7c11, -2*p7c11,-3*p7c11])

p7f1 = p7c1*x + p7c2
p7f2 = p7c3*y + p7c4
p7f3 = p7c5*z + p7c6
p7f4 = p7c7*x + p7c8
p7f5 = p7c9*y + p7c10
p7f6 = p7c11*z + p7c12

p7cc1 = NonZeroInt(-10,10, [0,1])
p7cc2 = NonZeroInt(-10,10, [0,1])
p7cc3 = NonZeroInt(-10,10, [0,1])
p7cc4 = NonZeroInt(-10,10, [0,1])
p7cc5 = NonZeroInt(-10,10, [0,1])
p7cc6 = NonZeroInt(-10,10, [0,1])

p7a1 = simplify(e^(p7cc1*ln(p7f1)+p7cc2*ln(p7f2)+p7cc3*ln(p7f3)+p7cc4*ln(p7f4)+p7cc5*ln(p7f5)+p7cc6*ln(p7f6)))


### Problem p8

p8b1 = NonZeroInt(2,15,[4,8,9])

p8c1 = NonZeroInt(-15,15)
p8c2 = NonZeroInt(-15,15,[0,p8c1, 2*p8c1, 3*p8c1, -p8c1, -2*p8c1,-3*p8c1])
p8c3 = NonZeroInt(-15,15)
p8c4 = NonZeroInt(-15,15,[0,p8c3, 2*p8c3, 3*p8c3, -p8c3, -2*p8c3,-3*p8c3])
p8c5 = NonZeroInt(-15,15)
p8c6 = NonZeroInt(-15,15,[0,p8c5, 2*p8c5, 3*p8c5, -p8c5, -2*p8c5,-3*p8c5])
p8c7 = NonZeroInt(-15,15,[0,p8c1])
p8c8 = NonZeroInt(-15,15,[0,p8c7, 2*p8c7, 3*p8c7, -p8c7, -2*p8c7,-3*p8c7])
p8c9 = NonZeroInt(-15,15,[0,p8c2])
p8c10 = NonZeroInt(-15,15,[0,p8c9, 2*p8c9, 3*p8c9, -p8c9, -2*p8c9,-3*p8c9])
p8c11 = NonZeroInt(-15,15,[0,p8c3])
p8c12 = NonZeroInt(-15,15,[0,p8c11, 2*p8c11, 3*p8c11, -p8c11, -2*p8c11,-3*p8c11])

p8f1 = p8c1*x + p8c2
p8f2 = p8c3*y + p8c4
p8f3 = p8c5*z + p8c6
p8f4 = p8c7*x + p8c8
p8f5 = p8c9*y + p8c10
p8f6 = p8c11*z + p8c12

p8cc1 = NonZeroInt(-10,10, [0,1])
p8cc2 = NonZeroInt(-10,10, [0,1])
p8cc3 = NonZeroInt(-10,10, [0,1])
p8cc4 = NonZeroInt(-10,10, [0,1])
p8cc5 = NonZeroInt(-10,10, [0,1])
p8cc6 = NonZeroInt(-10,10, [0,1])

p8a1 = simplify(e^(p8cc1*ln(p8f1)+p8cc2*ln(p8f2)+p8cc3*ln(p8f3)+p8cc4*ln(p8f4)+p8cc5*ln(p8f5)+p8cc6*ln(p8f6)))





\end{sagesilent}



\begin{problem}
    Fully expand the following logarithmic expression. (Hint: Don't factor out common factors from the linear terms, Xronos isn't that smart ... yet.)
    
    $
    \logOld_{\sage{p1b1}}\left(\dfrac{(\sage{p1f1})(\sage{p1f2})^2(\sage{p1f3})^3}{(\sage{p1f4})^4(\sage{p1f5})^5(\sage{p1f6})^6}\right)
    $
    
    \begin{tabular}{ll}
            \hspace{2cm} & $= \logOld_{\sage{p1b1}}\left(\answer{\sage{p1f1}}\right) + 2\logOld_{\sage{p1b1}}\left(\answer{\sage{p1f2}}\right) + 3\logOld_{\sage{p1b1}}\left(\answer{\sage{p1f3}}\right)$ \\ 
            & $-4\logOld_{\sage{p1b1}}\left(\answer{\sage{p1f4}}\right) - 5\logOld_{\sage{p1b1}}\left(\answer{\sage{p1f5}}\right) - 6\logOld_{\sage{p1b1}}\left(\answer{\sage{p1f6}}\right)$
    \end{tabular}
\end{problem}


\begin{problem}
    Fully expand the following logarithmic expression. (Hint: Don't factor out common factors from the linear terms, Xronos isn't that smart ... yet.)
    
    $
    \logOld_{\sage{p2b1}}\left(\dfrac{(\sage{p2f1})(\sage{p2f2})^2(\sage{p2f3})^3}{(\sage{p2f4})^4(\sage{p2f5})^5(\sage{p2f6})^6}\right)
    $
    
    \begin{tabular}{ll}
            \hspace{2cm} & $= \logOld_{\sage{p2b1}}\left(\answer{\sage{p2f1}}\right) + 2\logOld_{\sage{p2b1}}\left(\answer{\sage{p2f2}}\right) + 3\logOld_{\sage{p2b1}}\left(\answer{\sage{p2f3}}\right)$ \\ 
            & $-4\logOld_{\sage{p2b1}}\left(\answer{\sage{p2f4}}\right) - 5\logOld_{\sage{p2b1}}\left(\answer{\sage{p2f5}}\right) - 6\logOld_{\sage{p2b1}}\left(\answer{\sage{p2f6}}\right)$
    \end{tabular}
\end{problem}

\begin{problem}
    Fully expand the following logarithmic expression. (Hint: Don't factor out common factors from the linear terms, Xronos isn't that smart ... yet.)
    
    $
    \logOld_{\sage{p3b1}}\left(\dfrac{(\sage{p3f1})(\sage{p3f2})^2(\sage{p3f3})^3}{(\sage{p3f4})^4(\sage{p3f5})^5(\sage{p3f6})^6}\right)
    $
    
    \begin{tabular}{ll}
            \hspace{2cm} & $= \logOld_{\sage{p3b1}}\left(\answer{\sage{p3f1}}\right) + 2\logOld_{\sage{p3b1}}\left(\answer{\sage{p3f2}}\right) + 3\logOld_{\sage{p3b1}}\left(\answer{\sage{p3f3}}\right)$ \\ 
            & $-4\logOld_{\sage{p3b1}}\left(\answer{\sage{p3f4}}\right) - 5\logOld_{\sage{p3b1}}\left(\answer{\sage{p3f5}}\right) +\answer{-6}\logOld_{\sage{p3b1}}\left({\sage{p3f6}}\right)$
    \end{tabular}
\end{problem}


\begin{problem}
    Fully expand the following logarithmic expression. (Hint: Don't factor out common factors from the linear terms, Xronos isn't that smart ... yet.)
    
    $
    \logOld_{\sage{p4b1}}\left(\dfrac{(\sage{p4f1})(\sage{p4f2})^2(\sage{p4f3})^3}{(\sage{p4f4})^4(\sage{p4f5})^5(\sage{p4f6})^6}\right)
    $
    
    \begin{tabular}{ll}
            \hspace{2cm} & $= \logOld_{\sage{p4b1}}\left(\answer{\sage{p4f1}}\right) + 2\logOld_{\sage{p4b1}}\left(\answer{\sage{p4f2}}\right) + 3\logOld_{\sage{p4b1}}\left(\answer{\sage{p4f3}}\right)$ \\ 
            & $-4\logOld_{\sage{p4b1}}\left(\answer{\sage{p4f4}}\right) + \answer{-5}\logOld_{\sage{p4b1}}\left({\sage{p4f5}}\right) - 6\logOld_{\sage{p4b1}}\left(\answer{\sage{p4f6}}\right)$
    \end{tabular}
\end{problem}


\begin{problem}
    Fully condense the following logarithmic expression until there is only one logarithmic function remaining, with no coefficient. (Note: Formatting may look a little odd in order to get it to fit on a page correctly without getting crazy scroll bars everywhere)
    
    \begin{tabular}{lll}
        $(\sage{p5cc1})\logOld_{\sage{p5b1}}\left(\sage{p5f1}\right)$& $+ 
        (\sage{p5cc2})\logOld_{\sage{p5b1}}\left(\sage{p5f2}\right)$&$ + 
        (\sage{p5cc3})\logOld_{\sage{p5b1}}\left(\sage{p5f3}\right)$ \\
        &$+(\sage{p5cc4})\logOld_{\sage{p5b1}}\left(\sage{p5f4}\right)$&$ + 
        (\sage{p5cc5})\logOld_{\sage{p5b1}}\left(\sage{p5f5}\right)$ \\
        &$ + (\sage{p5cc6})\logOld_{\sage{p5b1}}\left(\sage{p5f6}\right)$
    \end{tabular}
    \[
        \logOld_{\sage{p5b1}}\left( \answer{\sage{p5a1}} \right)
    \]
\end{problem}



\begin{problem}
    Fully condense the following logarithmic expression until there is only one logarithmic function remaining, with no coefficient. (Note: Formatting may look a little odd in order to get it to fit on a page correctly without getting crazy scroll bars everywhere)
    
    \begin{tabular}{lll}
        $(\sage{p6cc1})\logOld_{\sage{p6b1}}\left(\sage{p6f1}\right)$& $+ 
        (\sage{p6cc2})\logOld_{\sage{p6b1}}\left(\sage{p6f2}\right)$&$ + 
        (\sage{p6cc3})\logOld_{\sage{p6b1}}\left(\sage{p6f3}\right)$ \\
        &$+(\sage{p6cc4})\logOld_{\sage{p6b1}}\left(\sage{p6f4}\right)$&$ + 
        (\sage{p6cc5})\logOld_{\sage{p6b1}}\left(\sage{p6f5}\right)$ \\
        &$ + (\sage{p6cc6})\logOld_{\sage{p6b1}}\left(\sage{p6f6}\right)$
    \end{tabular}
    \[
        \logOld_{\sage{p6b1}}\left( \answer{\sage{p6a1}} \right)
    \]
\end{problem}



\begin{problem}
    Fully condense the following logarithmic expression until there is only one logarithmic function remaining, with no coefficient. (Note: Formatting may look a little odd in order to get it to fit on a page correctly without getting crazy scroll bars everywhere)
    
    \begin{tabular}{lll}
        $(\sage{p7cc1})\logOld_{\sage{p7b1}}\left(\sage{p7f1}\right)$& $+ 
        (\sage{p7cc2})\logOld_{\sage{p7b1}}\left(\sage{p7f2}\right)$&$ + 
        (\sage{p7cc3})\logOld_{\sage{p7b1}}\left(\sage{p7f3}\right)$ \\
        &$+(\sage{p7cc4})\logOld_{\sage{p7b1}}\left(\sage{p7f4}\right)$&$ + 
        (\sage{p7cc5})\logOld_{\sage{p7b1}}\left(\sage{p7f5}\right)$ \\
        &$ + (\sage{p7cc6})\logOld_{\sage{p7b1}}\left(\sage{p7f6}\right)$
    \end{tabular}
    \[
        \logOld_{\sage{p7b1}}\left( \answer{\sage{p7a1}} \right)
    \]
\end{problem}



\begin{problem}
    Fully condense the following logarithmic expression until there is only one logarithmic function remaining, with no coefficient. (Note: Formatting may look a little odd in order to get it to fit on a page correctly without getting crazy scroll bars everywhere)
    
    \begin{tabular}{lll}
        $(\sage{p8cc1})\logOld_{\sage{p8b1}}\left(\sage{p8f1}\right)$& $+ 
        (\sage{p8cc2})\logOld_{\sage{p8b1}}\left(\sage{p8f2}\right)$&$ + 
        (\sage{p8cc3})\logOld_{\sage{p8b1}}\left(\sage{p8f3}\right)$ \\
        &$+(\sage{p8cc4})\logOld_{\sage{p8b1}}\left(\sage{p8f4}\right)$&$ + 
        (\sage{p8cc5})\logOld_{\sage{p8b1}}\left(\sage{p8f5}\right)$ \\
        &$ + (\sage{p8cc6})\logOld_{\sage{p8b1}}\left(\sage{p8f6}\right)$
    \end{tabular}
    \[
        \logOld_{\sage{p8b1}}\left( \answer{\sage{p8a1}} \right)
    \]
\end{problem}



%\begin{problem}
%    Expand the following exponential so that each exponent has at most one term.
%    
%    \begin{itemize}
%        \item $\sage{p7q1} 
%            = \answer{\sage{p7a1}} \cdot \sage{p7b1^p7b2}^{\answer{x^{\sage{p7r1}}}} \cdot  \sage{p7b1^p7b3}^{\answer{y^{\sage{p7r2}}}} \cdot \sage{p7b1^p7b4}^{\answer{z^{\sage{p7r3}}}}$
%        \item $\sage{p8q1} 
%            = \answer{\sage{p8a1}} \cdot \answer{\sage{p8b1^p8b2}}^{{x^{\sage{p8r1}}}} \cdot  \sage{p8b1^p8b3}^{\answer{y^{\sage{p8r2}}}} \cdot \answer{\sage{p8b1^p8b4}}^{{z^{\sage{p8r3}}}}$
%        \item $\sage{p9q1} 
%            = \answer{\sage{p9a1}} \cdot \sage{p9b1^p9b2}^{\answer{x^{\sage{p9r1}}}} \cdot  \answer{\sage{p9b1^p9b3}}^{y^{\answer{\sage{p9r2}}}} \cdot \sage{p9b1^p9b4}^{z^{\answer{\sage{p9r3}}}}$
%        \item $\sage{p10q1} 
%            = \answer{\sage{p10a1}} \cdot \sage{p10b1^p10b2}^{\answer{x^{\sage{p10r1}}}} \cdot  \sage{p10b1^p10b3}^{\answer{y^{\sage{p10r2}}}} \cdot \sage{p10b1^p10b4}^{\answer{z^{\sage{p7r3}}}}$
%    \end{itemize}
%\end{problem}


\end{document}