\documentclass{ximeraXloud}
%\usepackage{sagetex}
%\usepackage{amsfonts}
\title{Functions Practice 1}
\renewcommand{\text}[1]{#1}
\newcommand{\sagecheck}[2]{
    \ifthenelse{}{}{}\textit{}
    }
\begin{document}
\input{Useful-Sage-Macros}

\begin{sagesilent}
funcvec = [x, x^2, x^3]

#### Start of problem p1
p1choice1 = RandInt(0,2)
p1choice2 = RandInt(0,2)

p1c1 = NonZeroInt(-5,5)
p1c2 = RandInt(-5,5)
p1c3 = NonZeroInt(-5,5)
p1c4 = NonZeroInt(-5,5,[p1c2])
p1c5 = NonZeroInt(-5,5)
p1c6 = NonZeroInt(-5,5)
p1c7 = NonZeroInt(-5,5)
p1c8 = NonZeroInt(-5,5)
p1c9 = NonZeroInt(-5,5)
p1c10 = NonZeroInt(-5,5)



p1f1 = p1c1 * funcvec[p1choice1](x + p1c2)
p1f2 = p1c3 * funcvec[p1choice2](x + p1c4)

p1ans1 = p1f1 + p1f2
p1ans2 = p1f1 - p1f2
p1ans3 = p1f1 *p1f2
p1ans4 = p1f1/p1f2


#### Start of problem p2
p2choice1 = RandInt(0,2)
p2choice2 = RandInt(0,2)

p2c1 = NonZeroInt(-5,5)
p2c2 = RandInt(-5,5)
p2c3 = NonZeroInt(-5,5)
p2c4 = NonZeroInt(-5,5,[p2c2])
p2c5 = NonZeroInt(-5,5)
p2c6 = NonZeroInt(-5,5)
p2c7 = NonZeroInt(-5,5)
p2c8 = NonZeroInt(-5,5)
p2c9 = NonZeroInt(-5,5)
p2c10 = NonZeroInt(-5,5)



p2f1 = p2c1 * funcvec[p2choice1](x + p2c2)
p2f2 = p2c3 * funcvec[p2choice2](x + p2c4)

p2ans1 = p2f1 + p2f2
p2ans2 = p2f1 - p2f2
p2ans3 = p2f1 *p2f2
p2ans4 = p2f1/p2f2


#### Start of problem p3
p3choice1 = RandInt(0,2)
p3choice2 = RandInt(0,2)

p3c1 = NonZeroInt(-5,5)
p3c2 = RandInt(-5,5)
p3c3 = NonZeroInt(-5,5)
p3c4 = NonZeroInt(-5,5,[p3c2])
p3c5 = NonZeroInt(-5,5)
p3c6 = NonZeroInt(-5,5)
p3c7 = NonZeroInt(-5,5)
p3c8 = NonZeroInt(-5,5)
p3c9 = NonZeroInt(-5,5)
p3c10 = NonZeroInt(-5,5)



p3f1 = p3c1 * funcvec[p3choice1](x + p3c2)
p3f2 = p3c3 * funcvec[p3choice2](x + p3c4)

p3ans1 = p3f1 + p3f2
p3ans2 = p3f1 - p3f2
p3ans3 = p3f1 *p3f2
p3ans4 = p3f1/p3f2


#### Start of problem p4
p4choice1 = RandInt(0,2)
p4choice2 = RandInt(0,2)

p4c1 = NonZeroInt(-5,5)
p4c2 = RandInt(-5,5)
p4c3 = NonZeroInt(-5,5)
p4c4 = NonZeroInt(-5,5,[p4c2])
p4c5 = NonZeroInt(-5,5)
p4c6 = NonZeroInt(-5,5)
p4c7 = NonZeroInt(-5,5)
p4c8 = NonZeroInt(-5,5)
p4c9 = NonZeroInt(-5,5)
p4c10 = NonZeroInt(-5,5)



p4f1 = p4c1 * funcvec[p4choice1](x + p4c2)
p4f2 = p4c3 * funcvec[p4choice2](x + p4c4)

p4ans1 = p4f1 + p4f2
p4ans2 = p4f1 - p4f2
p4ans3 = p4f1 *p4f2
p4ans4 = p4f1/p4f2


\end{sagesilent}

\begin{problem}
Consider the functions $f(x) = \sage{p1f1}$ and $g(x) = \sage{p1f2}$. Compute the following:
\begin{itemize}
\item $\left(f+g\right)(x) = \answer{\sage{p1ans1}}$
\item $\left(f-g\right)(x) = \answer{\sage{p1ans2}}$
\item $\left(fg\right)(x) = \answer{\sage{p1ans3}}$
\item $\left(\frac{f}{g}\right)(x) = \answer{\sage{p1ans4}}$
\end{itemize}
\end{problem}


\begin{problem}
Consider the functions $f(x) = \sage{p2f1}$ and $g(x) = \sage{p2f2}$. Compute the following:
\begin{itemize}
\item $\left(f+g\right)(x) = \answer{\sage{p2ans1}}$
\item $\left(f-g\right)(x) = \answer{\sage{p2ans2}}$
\item $\left(fg\right)(x) = \answer{\sage{p2ans3}}$
\item $\left(\frac{f}{g}\right)(x) = \answer{\sage{p2ans4}}$
\end{itemize}
\end{problem}


\begin{problem}
Consider the functions $f(x) = \sage{p3f1}$ and $g(x) = \sage{p3f2}$. Compute the following:
\begin{itemize}
\item $\left(f+g\right)(x) = \answer{\sage{p3ans1}}$
\item $\left(f-g\right)(x) = \answer{\sage{p3ans2}}$
\item $\left(fg\right)(x) = \answer{\sage{p3ans3}}$
\item $\left(\frac{f}{g}\right)(x) = \answer{\sage{p3ans4}}$
\end{itemize}
\end{problem}


\begin{problem}
Consider the functions $f(x) = \sage{p4f1}$ and $g(x) = \sage{p4f2}$. Compute the following:
\begin{itemize}
\item $\left(f+g\right)(x) = \answer{\sage{p4ans1}}$
\item $\left(f-g\right)(x) = \answer{\sage{p4ans2}}$
\item $\left(fg\right)(x) = \answer{\sage{p4ans3}}$
\item $\left(\frac{f}{g}\right)(x) = \answer{\sage{p4ans4}}$
\end{itemize}
\end{problem}



\end{document}